lean/src/internal/redundant_leaves_can_be_removed_2/ant_implies.lean
@@ -1,0 +1,40 @@
+import tactic
+import ...definitions
+import ..helper_defs
+import data.finset
+import ..utils
+import data.list
+import data.bool
+import ..leaves_theory
+
+variable [GuardModule]
+open GuardModule
+
+def Ant.implies: Ant bool → Ant bool → Prop
+| (Ant.branch a_tr1 a_tr2) (Ant.branch b_tr1 b_tr2) := a_tr1.implies b_tr1 ∧ a_tr2.implies b_tr2
+| (Ant.diverge a a_tr) (Ant.diverge b b_tr) := (a → b) ∧ a_tr.implies b_tr
+| (Ant.leaf a a_leaf) (Ant.leaf b b_leaf) := (a → b) ∧ a_leaf = b_leaf
+| _ _ := false
+
+inductive Ant.implies2: Ant bool → Ant bool → Prop
+| leaf { a b: bool } { leaf } (h: a → b):
+    Ant.implies2 (Ant.leaf a leaf) (Ant.leaf b leaf)
+| branch { a_tr1 a_tr2 b_tr1 b_tr2 } (h1: Ant.implies2 a_tr1 b_tr1) (h2: Ant.implies2 a_tr2 b_tr2):
+    Ant.implies2 (Ant.branch a_tr1 a_tr2) (Ant.branch b_tr1 b_tr2)
+| diverge { a b: bool } { a_tr b_tr } (h1: Ant.implies2 a_tr b_tr) (h2: a → b):
+    Ant.implies2 (Ant.diverge a a_tr) (Ant.diverge b b_tr)
+
+notation a ⇒ b := Ant.implies2 a b
+
+def Ant.implies_equal_structure { a b: Ant bool } (h: a ⇒ b):
+    a.map (λ x, false) = b.map (λ x, false) :=
+begin
+    induction h;
+    simp [Ant.map, *],
+end
+
+def Ant.implies_same_leaves { a b: Ant bool } (h: a ⇒ b): a.leaves = b.leaves :=
+begin
+    have := congr_arg Ant.leaves (Ant.implies_equal_structure h),
+    finish [map_leaves_id],
+end
