lean/src/internal/redundant_leaves_can_be_removed_2/inactive.lean
@@ -1,0 +1,265 @@
+import tactic
+import ...definitions
+import ..helper_defs
+import data.finset
+import ..utils
+import data.list
+import data.bool
+import ..leaves_theory
+import ..gdt_eval
+
+open finset
+
+variable [GuardModule]
+open GuardModule
+
+def Gdt.mark_all_leaves_inactive: Gdt → Ant bool
+| (Gdt.leaf leaf) := Ant.leaf tt leaf 
+| (Gdt.branch tr1 tr2) := Ant.branch tr1.mark_all_leaves_inactive tr2.mark_all_leaves_inactive
+| (Gdt.grd (Grd.xgrd _) tr) := tr.mark_all_leaves_inactive
+| (Gdt.grd (Grd.bang _) tr) := Ant.diverge tt tr.mark_all_leaves_inactive
+
+@[simp]
+lemma Gdt.mark_all_leaves_inactive.inactive_leaves (gdt: Gdt):
+    gdt.mark_all_leaves_inactive.inactive_leaves = gdt.leaves :=
+begin
+    induction gdt;
+    try { cases gdt_grd };
+    simp [*, Gdt.leaves, Gdt.mark_all_leaves_inactive, Ant.inactive_leaves],
+end
+
+@[simp]
+lemma Gdt.mark_all_leaves_inactive.critical_leaf_sets (gdt: Gdt):
+    gdt.mark_all_leaves_inactive.critical_leaf_sets = ∅ :=
+begin
+    induction gdt;
+    try { cases gdt_grd };
+    simp [*, Gdt.leaves, Gdt.mark_all_leaves_inactive, Ant.critical_leaf_sets],
+end
+
+@[simp]
+lemma Gdt.mark_all_leaves_inactive.leaves (gdt: Gdt):
+    gdt.mark_all_leaves_inactive.leaves = gdt.leaves :=
+begin
+    induction gdt;
+    try { cases gdt_grd };
+    simp [*, Gdt.leaves, Gdt.mark_all_leaves_inactive, Ant.critical_leaf_sets, Ant.leaves],
+end
+
+@[simp]
+lemma Gdt.mark_all_leaves_inactive_map_false (gdt: Gdt):
+    gdt.mark_all_leaves_inactive.map (λ x, tt) = gdt.mark_all_leaves_inactive :=
+begin
+    induction gdt;
+    try { cases gdt_grd };
+    simp [*, Ant.map, Gdt.mark_all_leaves_inactive],
+end
+
+def Gdt.mark_inactive_leaves : Gdt → Env → Ant bool
+| (Gdt.leaf leaf) env := Ant.leaf ff leaf 
+| (Gdt.branch tr1 tr2) env :=
+    if (tr1.eval env).is_match then
+        Ant.branch (tr1.mark_inactive_leaves env) (tr2.mark_all_leaves_inactive)
+    else
+        Ant.branch (tr1.mark_all_leaves_inactive) (tr2.mark_inactive_leaves env)
+| (Gdt.grd (Grd.xgrd grd) tr) env :=
+    match xgrd_eval grd env with
+    | none := tr.mark_all_leaves_inactive
+    | some env' := tr.mark_inactive_leaves env'
+    end
+| (Gdt.grd (Grd.bang var) tr) env :=
+    if is_bottom var env
+    then Ant.diverge ff (tr.mark_all_leaves_inactive)
+    else Ant.diverge tt (tr.mark_inactive_leaves env)
+
+lemma Gdt.mark_inactive_leaves_mark_all_leaves_inactive (gdt: Gdt) (env: Env):
+    (gdt.mark_inactive_leaves env).map (λ x, tt) = gdt.mark_all_leaves_inactive :=
+begin
+    induction gdt generalizing env;
+    try { cases gdt_grd };
+    try { cases c: (gdt_tr1.eval env).is_match };
+    try { cases c: (xgrd_eval gdt_grd env) };
+    try { cases c: is_bottom gdt_grd env };
+    simp [*, Gdt.leaves, Gdt.mark_inactive_leaves, Gdt.mark_all_leaves_inactive, Ant.leaves, Ant.map],
+end
+
+@[simp]
+lemma Gdt.mark_inactive_leaves.leaves (gdt: Gdt) (env: Env):
+    (gdt.mark_inactive_leaves env).leaves = gdt.leaves :=
+begin
+    induction gdt generalizing env;
+    try { cases gdt_grd };
+    try { cases c: (gdt_tr1.eval env).is_match };
+    try { cases c: (xgrd_eval gdt_grd env) };
+    try { cases c: is_bottom gdt_grd env };
+    simp [*, Gdt.leaves, Gdt.mark_inactive_leaves, Ant.critical_leaf_sets, Ant.leaves],
+end
+
+
+lemma Gdt.mark_inactive_leaves_no_match { env: Env } { gdt: Gdt } (h: gdt.eval env = Result.no_match):
+    gdt.mark_inactive_leaves env = gdt.mark_all_leaves_inactive :=
+begin
+    induction gdt with leaf generalizing env,
+    case Gdt.leaf {
+        finish [Gdt.eval],
+    },
+    case Gdt.branch {
+        simp [
+            Gdt.mark_inactive_leaves, Gdt.mark_all_leaves_inactive,
+            gdt_eval_branch_no_match.1 h, *
+        ],
+    },
+    case Gdt.grd {
+        cases gdt_grd with gdt_grd var,
+        case Grd.xgrd {
+            cases c: xgrd_eval gdt_grd env, {
+                simp [Gdt.mark_inactive_leaves, Gdt.mark_all_leaves_inactive, c],
+            }, {
+                rw [grd_eval_xgrd_some c] at h,
+                simp [Gdt.mark_inactive_leaves, Gdt.mark_all_leaves_inactive, c, gdt_ih h],
+            },
+        },
+        case Grd.bang {
+            simp [Gdt.mark_inactive_leaves, Gdt.mark_all_leaves_inactive, grd_eval_bang_no_match.1 h, gdt_ih],
+        }
+    }
+end
+
+lemma sets_1 { α: Type } [decidable_eq α] { l1 l2 l3 l4: finset α }
+    (h1: l4 ∩ (l1 ∪ l2) ⊆ l1 ∪ l3)
+    (h2: disjoint l1 l2)
+    : l4 ∩ l2 ⊆ l3 :=
+begin
+    rw finset.subset_iff,
+    simp,
+    assume x h3 h4,
+
+    rw finset.subset_iff at h1,
+    specialize @h1 x,
+    simp at h1,
+
+    simp [finset.disjoint_iff_inter_eq_empty, finset.subset.antisymm_iff, finset.subset_iff] at h2,
+    specialize @h2 x,
+
+    tauto, 
+end
+
+lemma sets_2 { α: Type } [decidable_eq α] { l1 l2 l3 l4: finset α }
+    (h1: l4 ∩ (l1 ∪ l2) ⊆ l3 ∪ l2)
+    (h2: disjoint l1 l2)
+    : l4 ∩ l1 ⊆ l3 :=
+begin
+    rw finset.subset_iff,
+    simp,
+    assume x h3 h4,
+
+    rw finset.subset_iff at h1,
+    specialize @h1 x,
+    simp at h1,
+
+    simp [finset.disjoint_iff_inter_eq_empty, finset.subset.antisymm_iff, finset.subset_iff] at h2,
+    specialize @h2 x,
+
+    tauto, 
+end
+
+lemma inactive_leaves_can_be_removed
+    (gdt: Gdt) (gdt_disjoint: gdt.disjoint_leaves)
+    -- We only focus on a very particular environment `env`.
+    (env: Env)
+    
+    (leaves: finset Leaf) (leaves_def: can_be_removed (gdt.mark_inactive_leaves env) leaves):
+
+        Gdt.eval_option (gdt.remove_leaves leaves) env = gdt.eval env :=
+begin
+  induction gdt with leaf generalizing env,
+  case Gdt.leaf {
+      simp [Gdt.eval],
+      unfold Gdt.mark_inactive_leaves can_be_removed at leaves_def,
+      simp [Ant.inactive_leaves, Ant.critical_leaf_sets] at leaves_def,
+      sorry,
+  },
+
+  case Gdt.branch {
+        simp [Gdt.mark_inactive_leaves] at leaves_def,
+        cases (gdt_tr1.eval env).is_match,
+        case bool.ff {
+            simp [Ant.inactive_leaves, Gdt.mark_inactive_leaves, can_be_removed, Ant.critical_leaf_sets ] at leaves_def,
+            simp [Ant.leaves] at leaves_def,
+
+            unfold Gdt.remove_leaves,
+            unfold Gdt.disjoint_leaves at gdt_disjoint,
+
+            have : can_be_removed (gdt_tr2.mark_inactive_leaves env) leaves :=
+            begin
+                have := sets_1 leaves_def.1 gdt_disjoint.2.2,
+                unfold can_be_removed,
+                split, { simp [*], },
+                exact leaves_def.2,
+            end,
+
+            specialize gdt_ih_tr2 gdt_disjoint.2.1 env this,
+            sorry,
+        },
+        case bool.tt {
+            simp [Ant.inactive_leaves, Gdt.mark_inactive_leaves, can_be_removed, Ant.critical_leaf_sets ] at leaves_def,
+            simp [Ant.leaves] at leaves_def,
+
+            unfold Gdt.remove_leaves,
+            unfold Gdt.disjoint_leaves at gdt_disjoint,
+
+            have : can_be_removed (gdt_tr1.mark_inactive_leaves env) leaves :=
+            begin
+                unfold can_be_removed,
+                simp,
+                have := sets_2 leaves_def.1 gdt_disjoint.2.2,
+                split, { simp [*], },
+                exact leaves_def.2,
+            end,
+            specialize gdt_ih_tr1 gdt_disjoint.1 env this,
+            sorry,
+        },
+    },
+
+    case Gdt.grd {
+        unfold Gdt.disjoint_leaves at gdt_disjoint,
+        cases gdt_grd with gdt_grd var,
+        case Grd.xgrd {
+            cases c: xgrd_eval gdt_grd env with env',
+            case option.some {
+                simp [grd_eval_xgrd_some c],
+                unfold can_be_removed at leaves_def,
+                simp only [Gdt.mark_inactive_leaves, Gdt.mark_inactive_leaves._match_1, c] at leaves_def,
+                rw ←can_be_removed at leaves_def,
+                specialize gdt_ih gdt_disjoint env' leaves_def,
+                unfold Gdt.remove_leaves,
+                sorry,
+            },
+            case option.none {
+                simp [grd_eval_xgrd_none c],
+                unfold Gdt.remove_leaves,
+                sorry,
+            },
+        },
+        case Grd.bang {
+            cases c: is_bottom var env,
+            case bool.tt {
+                simp [grd_eval_bang_bottom c],
+                simp [can_be_removed, Gdt.leaves, Ant.leaves, Ant.inactive_leaves, Ant.critical_leaf_sets, Gdt.mark_inactive_leaves, c] at leaves_def,
+                unfold Gdt.remove_leaves,
+                sorry,
+            },
+            case bool.ff {
+                simp [can_be_removed, Gdt.leaves, Gdt.mark_inactive_leaves, c, Ant.leaves, Ant.inactive_leaves, Ant.critical_leaf_sets] at leaves_def,
+                have : can_be_removed (gdt_tr.mark_inactive_leaves env) leaves, {
+                    simp [can_be_removed, Gdt.leaves, Gdt.mark_inactive_leaves, c, Ant.leaves, Ant.inactive_leaves, Ant.critical_leaf_sets],
+                    exact leaves_def,
+                },
+                specialize gdt_ih gdt_disjoint env this,
+                unfold Gdt.remove_leaves,
+                simp [grd_eval_bang_not_bottom c],
+                sorry,
+            },
+        },
+    },
+end
