lean/src/internal/redundant_leaves_can_be_removed_2/main.lean
@@ -1,0 +1,320 @@
+import tactic
+import data.finset
+import data.list
+import data.bool
+import ...definitions
+import ..helper_defs
+import ..utils
+import ..leaves_theory
+import .ant_implies
+import .inactive
+import ..U_semantic
+
+variable [GuardModule]
+open GuardModule
+
+
+def Ant.mark_inactive_leaves (ant: Ant Φ) (env: Env) := ant.map (λ ty, !(ty.eval env))
+
+@[simp]
+lemma Ant.mark_inactive_leaves.branch (ant1 ant2: Ant Φ) (env) :
+    (ant1.branch ant2).mark_inactive_leaves env = (ant1.mark_inactive_leaves env).branch (ant2.mark_inactive_leaves env) :=
+by simp [Ant.map, Ant.mark_inactive_leaves]
+
+@[simp]
+lemma Ant.mark_inactive_leaves.diverge (a) (ant: Ant Φ) (env) :
+    (Ant.diverge a ant).mark_inactive_leaves env = Ant.diverge (!(a.eval env)) (ant.mark_inactive_leaves env) :=
+by simp [Ant.map, Ant.mark_inactive_leaves]
+
+lemma can_prove_empty_implies_inactive { can_prove_empty: Gs } { ant: Ant Φ } { env: Env }:
+    (ant.map (can_prove_empty.val)) ⇒ (ant.mark_inactive_leaves env) :=
+begin
+    induction ant,
+    case Ant.leaf {
+        unfold Ant.map Ant.mark_inactive_leaves,
+        apply Ant.implies2.leaf,
+        -- TODO WTF
+        unfold_coes,
+        simp,
+        unfold_coes,
+        apply is_empty_implies_eval_false,
+    },
+    case Ant.branch {
+        -- TODO only is required here
+        simp only [Ant.implies2.branch, Ant.map, *, Ant.mark_inactive_leaves.branch],
+    },
+    case Ant.diverge {
+        unfold Ant.map,
+        rw Ant.mark_inactive_leaves.diverge,
+        apply Ant.implies2.diverge,
+        { exact ant_ih, },
+        {
+            -- TODO can this be improved?
+            have := @is_empty_implies_eval_false _ can_prove_empty ant_a env,
+            unfold_coes,
+            finish,
+        }
+    },
+end
+
+lemma A_mark_inactive_leaves (gdt: Gdt) (env: Env): (A gdt).mark_inactive_leaves env = gdt.mark_inactive_leaves env :=
+begin
+    induction gdt generalizing env,
+    case Gdt.leaf {
+        simp [A, Ant.mark_inactive_leaves, Ant.map, Φ.eval, Gdt.mark_inactive_leaves],
+    },
+    case Gdt.branch {
+        unfold A Ant.mark_inactive_leaves Ant.map Gdt.mark_inactive_leaves,
+        rw Ant.map.associative,
+        rw function.comp,
+        unfold Φ.eval,
+        rw U_semantic,
+
+        cases c: (gdt_tr1.eval env).is_match,
+        case bool.ff {
+            have : gdt_tr1.eval env = Result.no_match, { cases gdt_tr1.eval env; finish, },
+            specialize gdt_ih_tr1 env,
+            unfold Ant.mark_inactive_leaves at gdt_ih_tr1,
+            specialize gdt_ih_tr2 env,
+            unfold Ant.mark_inactive_leaves at gdt_ih_tr2,
+            
+            simp [c, ←Gdt.mark_inactive_leaves_no_match this, *],
+        },
+
+        case bool.tt {
+            have : (A gdt_tr2).map (λ (x : Φ), !(!tt && x.eval env)) =
+                    (((A gdt_tr2).mark_inactive_leaves env).map (λ x, tt)) := 
+            begin
+                simp [Ant.mark_inactive_leaves, Ant.map.associative, function.comp],
+            end,
+            rw this,
+            specialize gdt_ih_tr2 env,
+            rw gdt_ih_tr2,
+            specialize gdt_ih_tr1 env,
+            unfold Ant.mark_inactive_leaves at gdt_ih_tr1,
+            simp [Gdt.mark_inactive_leaves_mark_all_leaves_inactive, *],
+        },
+    },
+    case Gdt.grd {
+        cases gdt_grd,
+        case Grd.xgrd {
+            unfold A Ant.map,
+            unfold Ant.mark_inactive_leaves,
+            rw Ant.map.associative,
+            rw function.comp,
+            unfold Φ.eval,
+
+            unfold Gdt.mark_inactive_leaves,
+
+            cases xgrd_eval gdt_grd env;
+
+            unfold Gdt.mark_inactive_leaves._match_1;
+            unfold Φ.eval._match_1,
+
+            {
+                have := Gdt.mark_inactive_leaves_mark_all_leaves_inactive gdt_tr env,
+                rw ←gdt_ih at this,
+                rw Ant.mark_inactive_leaves at this,
+                rw Ant.map.associative at this,
+                rw function.comp at this,
+                simp [this],
+            },
+            {
+                rw ←gdt_ih val,
+                rw ←Ant.mark_inactive_leaves,
+            },
+        },
+        case Grd.bang {
+
+        },
+        simp [A, Ant.mark_inactive_leaves, Ant.map, Φ.eval, Gdt.mark_inactive_leaves],
+        
+    },
+end
+
+/-
+lemma redundant_implies_inactive
+    (gdt: Gdt) (can_prove_empty: Gs) (env: Env)
+    (ant: Ant Φ) (ant_def: ant.eval_leaves = (A gdt).eval_leaves):
+    (ant.map (can_prove_empty.val)).implies (Gdt.mark_inactive_leaves gdt env) :=
+begin
+    induction gdt generalizing env,
+    case Gdt.leaf {
+        rw A at ant_def,
+        replace ant_def := congr_fun ant_def env,
+        unfold Ant.eval_leaves at ant_def,
+        rw map_ant_structure_leaf ant ant_def,
+        
+        simp [Ant.implies, Ant.map, Gdt.mark_inactive_leaves],
+    },
+    sorry,
+end
+-/
+
+lemma removable_monotonous' { a b: Ant bool } (h: a ⇒ b): 
+        a.inactive_leaves ⊆ b.inactive_leaves ∧ b.critical_leaf_sets ⊆ a.critical_leaf_sets :=
+begin
+    induction a generalizing b;
+    cases h with h b_a,
+    -- case leaf:
+    {
+        cases a_a; cases b_a;
+        finish [Ant.inactive_leaves, Ant.implies2.leaf],
+    },
+    -- case branch:
+    {
+        specialize a_ih_tr1 h_h1,
+        specialize a_ih_tr2 h_h2,
+        simp [ *, finset.union_subset_union, Ant.inactive_leaves, Ant.critical_leaf_sets ],
+    },
+    -- case grd:
+    {
+        specialize a_ih h_h1,
+        split, { simp [Ant.inactive_leaves, a_ih], },
+
+        cases a_a; cases h_b;
+        finish [
+            Ant.critical_leaf_sets,
+            Ant.implies_same_leaves h_h1,
+            finset.union_subset_union,
+            a_ih.2,
+            subset_right_union
+        ],
+    },
+end
+
+lemma removable_monotonous { a b: Ant bool } (leaves: finset Leaf) (h: a ⇒ b):
+    removable a leaves → removable b leaves :=
+begin
+    unfold removable,
+    have := removable_monotonous' h,
+    assume p,
+    split,
+    {
+        rw ←Ant.implies_same_leaves h,
+        exact finset.subset.trans p.1 this.1,
+    },
+    assume e,
+    assume q,
+    exact p.right e (this.2 q),
+end
+
+lemma R'_red_removable (ant: Ant bool)
+    --(ant_disjoint: ant.disjoint_leaves)
+    : removable ant (R' ant).red.to_finset :=
+begin
+    induction ant,
+
+    case Ant.leaf {
+        unfold removable R',
+        cases ant_a;
+        simp [Ant.critical_leaf_sets, Ant.inactive_leaves, Ant.leaves],
+    },
+    case Ant.branch {
+        unfold removable R',
+        unfold removable R' at ant_ih_tr1,
+        unfold removable R' at ant_ih_tr2,
+        unfold LeafPartition.red,
+        split, {
+            simp [Ant.inactive_leaves, finset.union_subset_union ant_ih_tr1.1 ant_ih_tr2.1, Ant.leaves],
+            sorry,
+        },
+
+        assume e,
+        assume h,
+        rw Ant.critical_leaf_sets at h,
+        
+        simp,
+        sorry,
+    },
+    case Ant.diverge {
+        unfold removable,
+        unfold removable at ant_ih,
+
+        split, {
+            cases R_diverge ant_a (refl (R' ant_tr)) with d d,
+            case or.inl {
+                cases d with leaf d,
+                cases d with ls d,
+                rw d.2.2,
+                unfold LeafPartition.red,
+                rw d.2.1 at ant_ih,
+                unfold LeafPartition.red at ant_ih,
+                unfold Ant.inactive_leaves,
+                sorry,
+            },
+            case or.inr {
+                simp [d.2, Ant.inactive_leaves, ant_ih.1],
+                sorry,
+            },
+        },
+
+        assume e,
+        assume h,
+
+
+        unfold Ant.critical_leaf_sets at h,
+
+        cases R_diverge ant_a (refl (R' ant_tr)) with d d,
+        case or.inr {
+            rw d.2,
+            sorry,
+        },
+
+        case or.inl {
+            cases d with leaf d,
+            cases d with ls d,
+            rw d.1 at h,
+            simp at h,
+            rw d.2.2,
+            unfold LeafPartition.red,
+            rw d.2.1 at ant_ih,
+            unfold LeafPartition.red at ant_ih,
+            sorry,
+        },
+    },
+end
+
+theorem redundant_leaves_removable
+    (can_prove_empty: Gs)
+    (gdt: Gdt) (gdt_disjoint: gdt.disjoint_leaves):
+    Gdt.eval_option (gdt.remove_leaves ((R can_prove_empty.val (A gdt)).red.to_finset)) = gdt.eval :=
+begin
+    ext env:1,
+    
+    -- `A gdt` represents `gdt` by annotating it with refinement types.
+    -- `can_prove_empty` approximates emptiness for a single refinement type.
+    let ant := (A gdt).map can_prove_empty.val,
+
+    -- `ant` approximates emptiness of these refinement types (s1).
+    have s1: ant ⇒ (A gdt).mark_inactive_leaves env
+        := @can_prove_empty_implies_inactive _ can_prove_empty (A gdt) env,
+
+    -- Since a refinement type in `A gdt` is empty in `env` iff
+    -- the corresponding leaf- or diverge-node in `gdt` is inactive in `env` (s2),
+    have s2: (A gdt).mark_inactive_leaves env = gdt.mark_inactive_leaves env
+        := A_mark_inactive_leaves gdt env,
+    -- `ant` also approximates inactive leaves of `gdt` in context of `env` (s3).
+    have s3: ant ⇒ gdt.mark_inactive_leaves env
+        := eq.subst s2 s1,
+    
+    
+    let R'_red_leaves := (R' ant).red.to_finset,
+
+    -- The set of leaves `R'_red_leaves` can be removed from `ant`.
+    -- This means that these leaves are inactive
+    -- and possibly active diverge nodes are not removed.
+    have s4: removable ant R'_red_leaves
+        := R'_red_removable
+     ant,
+    
+    -- Since `removable` is monotonous and `ant` approximates inactive leaves on `gdt`,
+    -- `R'_red_leaves` can also be removed from `gdt`.
+    have: R'_red_leaves.removable (gdt.mark_inactive_leaves env)
+        := removable_monotonous _ s3 s4,
+    
+    have: Gdt.eval_option (Gdt.remove_leaves R'_red_leaves gdt) env = gdt.eval env
+        := inactive_leaves_removable gdt gdt_disjoint env _ this,
+
+    exact this,
+end
